src/Scoping.v
@@ -101,7 +101,7 @@ Combined Scheme scoped_ind from ValScoped_ind2, ExpScoped_ind2.
 Check scoped_ind.
 
 Definition subst_preserves (Γ : nat) (ξ : Substitution) : Prop :=
-  forall v, v < Γ -> ξ v = None.
+  forall v, v < Γ -> ξ v = inr v.
 
 Theorem subst_preserves_up : forall Γ ξ,
   subst_preserves Γ ξ -> subst_preserves (S Γ) (up_subst ξ).
@@ -177,70 +177,6 @@ Proof.
   intros. pose (scoped_ignores_sub 0). destruct a. apply H0; auto.
 Qed.
 
-(* Theorem scope_duplicate e :
-  (forall Γ v, v < Γ -> EXP (S Γ) ⊢ e -> EXP Γ ⊢ e) /\
-  (forall Γ v, v < Γ -> VAL (S Γ) ⊢ e -> VAL Γ ⊢ e).
-Proof.
-  einduction e using Exp_ind2 with 
-      (Q := fun l => Forall (fun e => 
-        (forall Γ v, v < Γ -> EXP (S Γ) ⊢ e -> EXP Γ ⊢ e) /\
-        (forall Γ v, v < Γ -> VAL (S Γ) ⊢ e -> VAL Γ ⊢ e)) l); intros.
-  * repeat constructor.
-  * split; intros.
-    - inversion H0. subst. inversion H1. constructor. subst. inversion H3; subst;
-      constructor; auto.
-    - inversion H0. inversion H2; subst; constructor; auto.
-  * split; intros. 
-    - inversion H0. subst. inversion H1. inversion H3; constructor; subst;
-      constructor; auto.
-    - inversion H0. inversion H2; subst; constructor; auto.
-  * split; intros. 
-    - constructor. constructor. inversion H0. inversion H1. subst.
-      rewrite <- app_comm_cons in H4. apply IHe0 in H4; auto. apply in_or_app. left.
-      auto.
-    - constructor. inversion H0. subst.
-      rewrite <- app_comm_cons in H2. apply IHe0 in H2; auto. apply in_or_app. left.
-      auto.
-  * split; intros. 
-    - constructor. constructor. inversion H0. inversion H1. subst.
-      rewrite <- app_comm_cons in H4. apply IHe0 in H4; auto. apply in_or_app. left.
-      auto.
-    - constructor. inversion H0. subst.
-      rewrite <- app_comm_cons in H2. apply IHe0 in H2; auto. apply in_or_app. left.
-      auto.
-  * split; intros; inversion H0. 2: inversion H1. subst. rewrite indexed_to_forall in IHe1.
-    constructor.
-    - eapply IHe0; eauto.
-    - intros. eapply IHe1; eauto.
-  * split; intros; inversion H0. 2: inversion H1. subst. constructor.
-    - eapply IHe0_1. exact H. auto.
-    - rewrite <- app_comm_cons in H5. eapply IHe0_2. 2: exact H5.
-      apply in_or_app. left. auto.
-  * split; intros; inversion H0. 2: inversion H1. subst. constructor.
-    - eapply IHe0_1. apply in_or_app. left. eauto. rewrite <- app_comm_cons in H3. auto.
-    - eapply IHe0_2. apply in_or_app. left. eauto. rewrite <- app_comm_cons in H6. auto.
-  * split; intros; inversion H0. 2: inversion H1. subst. constructor.
-    - eapply IHe0_1; eauto.
-    - eapply IHe0_2; eauto.
-  * split; intros; inversion H0. 2: inversion H1. subst. constructor.
-    - eapply IHe0_1; eauto.
-    - eapply IHe0_2; eauto.
-    - eapply IHe0_3; eauto.
-  * constructor; eauto.
-  * constructor.
-Qed.
-
-Require Import Sorting.Permutation.
-
-Theorem perm_scoped : forall Γ,
-  (forall e, VAL Γ ⊢ e -> forall Γ', Permutation Γ Γ' -> VAL Γ' ⊢ e) /\
-  (forall e, EXP Γ ⊢ e -> forall Γ', Permutation Γ Γ' ->  EXP Γ' ⊢ e).
-Proof.
-  apply scoped_ind; intros; constructor; intuition.
-  1-2: eapply Permutation_in; eauto.
-  all: apply H0 || apply H; apply Permutation_app; intuition.
-Qed. *)
-
 Theorem scope_ext : forall Γ,
   (forall e, VAL Γ ⊢ e ->  VAL (S Γ) ⊢ e) /\
   forall e, EXP Γ ⊢ e -> EXP (S Γ) ⊢ e.
@@ -249,337 +185,725 @@ Proof.
   all: rewrite Nat.add_succ_r; auto.
 Qed.
 
+Lemma scope_ext_Exp : forall {e Γ},
+    EXP Γ ⊢ e -> EXP S Γ ⊢ e.
+Proof.
+  intros.
+  apply scope_ext.
+  auto.
+Qed.
+
+Lemma scope_ext_Val : forall {e Γ},
+    VAL Γ ⊢ e -> VAL S Γ ⊢ e.
+Proof.
+  intros.
+  apply scope_ext.
+  auto.
+Qed.
+
 Theorem app_cons_swap {T : Type} : forall (l l' : list T) (a : T),
   l ++ a::l' = l ++ [a] ++ l'.
 Proof.
   firstorder.
 Qed.
 
-Corollary scope_ext_app : forall l Γ,
-  (forall e, VAL Γ ⊢ e -> VAL Γ ++ l ⊢ e) /\
-  forall e, EXP Γ ⊢ e -> EXP Γ ++ l ⊢ e.
+Corollary scope_ext_app : forall Γ' Γ, Γ <= Γ' ->
+  (forall e, VAL Γ ⊢ e -> VAL Γ' ⊢ e) /\
+  forall e, EXP Γ ⊢ e -> EXP Γ' ⊢ e.
 Proof.
- induction l; intros.
- * repeat rewrite app_nil_r. split; intros; auto.
- * rewrite app_cons_swap. pose (scope_ext Γ). specialize (IHl (Γ ++ [a])).
-   destruct IHl, a0. split; intros.
-   - specialize (H1 e H3 a). eapply perm_scoped in H1. rewrite app_assoc.
-     apply H. exact H1. apply Permutation_cons_append.
-   - specialize (H2 e H3 a). eapply perm_scoped in H2. rewrite app_assoc.
-     apply H0. exact H2. apply Permutation_cons_append.
+ intros. induction H.
+ * intuition.
+ * split; intros; eapply scope_ext; eapply IHle; auto. 
 Qed.
 
-(*
-Theorem scope_subst v : forall e,
-  (forall Γ, VAL (inl v::Γ) ⊢ e -> forall val, VAL Γ ⊢ val -> VAL Γ ⊢ (varsubst v val e)) /\
-  (forall Γ, EXP (inl v::Γ) ⊢ e -> forall val, EXP Γ ⊢ val -> EXP Γ ⊢ (varsubst v val e)).
+Definition subscoped (Γ Γ' : nat) (ξ : Substitution) : Prop :=
+  forall v, v < Γ -> (match ξ v with
+                      | inl exp => VAL Γ' ⊢ exp
+                      | inr num => num < Γ'  (* in case of identity subst *)
+                      end).
+
+Notation "'SUBSCOPE' Γ ⊢ ξ ∷ Γ'" := (subscoped Γ Γ' ξ)
+         (at level 69, ξ at level 99, no associativity).
+
+Definition renscoped (Γ : nat) (Γ' : nat) (ξ : Renaming) : Prop :=
+  forall v, v < Γ -> (ξ v) < Γ'.
+
+Notation "'RENSCOPE' Γ ⊢ ξ ∷ Γ'" := (renscoped Γ Γ' ξ)
+         (at level 69, ξ at level 99, no associativity).
+
+Lemma renscope_id Γ : RENSCOPE Γ ⊢ id ∷ Γ.
 Proof.
-  einduction e using Exp_ind2 with 
-  (Q := fun l => Forall (fun e => (forall Γ, VAL (inl v::Γ) ⊢ e -> forall val, VAL Γ ⊢ val -> VAL Γ ⊢ (varsubst v val e)) /\
-  (forall Γ, EXP (inl v::Γ) ⊢ e -> forall val, EXP Γ ⊢ val -> EXP Γ ⊢ (varsubst v val e))) l); intros.
-  * split; intros; simpl; constructor. constructor.
-  * split; intros;
-    subst; simpl; break_match_goal.
-    - apply eqb_eq in Heqb. subst. simpl. auto.
-    - apply eqb_neq in Heqb. inversion H. inversion H2. congruence.
-      constructor. auto.
-    - apply eqb_eq in Heqb. subst. simpl. auto.
-    - apply eqb_neq in Heqb. inversion H. inversion H1. inversion H4. congruence.
-      constructor. constructor. auto.
-  * split; intros. inversion H.
-    - subst. simpl. inversion H2. inversion H1. constructor. auto.
-    - subst. simpl. inversion H. inversion H1. constructor. constructor.
-      inversion H4; auto. congruence.
-  * split; intros; inversion H; subst; simpl; break_match_goal; constructor.
-    3-4: constructor.
-    - apply in_list_sound in Heqb. rewrite <- app_comm_cons in H2.
-      eapply scope_duplicate in H2; auto. apply in_app_iff. right. apply in_map. auto.
-    - apply IHe0. rewrite <- app_comm_cons in H2. auto.
-      eapply scope_ext_app. constructor. auto.
-    - apply in_list_sound in Heqb. inversion H1; subst. 
-      rewrite <- app_comm_cons in H3.
-      eapply scope_duplicate in H3; auto. apply in_app_iff. right. apply in_map. auto.
-    - inversion H1. subst. apply IHe0. rewrite app_comm_cons. auto.
-      eapply scope_ext_app. auto.
-  * split; intros; inversion H; subst; simpl; break_match_goal; constructor.
-    3-4: constructor.
-    - apply in_list_sound in Heqb. rewrite <- app_comm_cons in H2.
-      eapply scope_duplicate in H2; auto. apply in_app_iff. right.
-      apply in_app_iff. right. apply in_map. auto.
-    - apply IHe0. rewrite <- app_comm_cons in H2. auto.
-      eapply scope_ext_app. constructor. auto.
-    - apply in_list_sound in Heqb. inversion H1; subst. 
-      rewrite <- app_comm_cons in H3.
-      eapply scope_duplicate in H3; auto. apply in_app_iff. right.
-      apply in_app_iff. right. apply in_map. auto.
-    - inversion H1. subst. apply IHe0. rewrite app_comm_cons. auto.
-      eapply scope_ext_app. auto.
-  * split; intros. inversion H.
-    simpl. inversion H. 2: inversion H1. subst. constructor.
-    - apply IHe0. auto. auto.
-    - rewrite indexed_to_forall in IHe1.
-      intros. epose (IHe1 i _). destruct a. clear H2 IHe1. Search map nth.
-      replace (ELit 0) with ((varsubst v val) (ELit 0)). rewrite map_nth. apply H5.
-      apply H4. rewrite map_length in H1. auto. auto. reflexivity.
-  * split; intros; inversion H; subst.
-    - simpl. break_match_goal.
-      + apply eqb_eq in Heqb. subst. constructor. apply IHe0_1; eauto.
-        apply scope_duplicate in H5. 2: apply in_or_app; right; constructor; auto.
-        exact H5.
-      + apply eqb_neq in Heqb. constructor.
-        apply IHe0_1; eauto.
-        apply IHe0_2; eauto.
-        eapply scope_ext_app in H0. eauto.
-    - inversion H1.
-  * split; intros. inversion H. subst.
-    simpl. inversion H. 2: inversion H1. subst. break_match_goal.
-    - constructor. rewrite <- app_comm_cons in H3. eapply scope_duplicate.
-      2: exact H3. apply in_list_sound in Heqb. apply in_app_iff. right.
-      apply in_app_iff. right.
-      apply in_map. auto.
-      apply IHe0_2. rewrite <- app_comm_cons in H6. auto.
-      eapply scope_ext_app in H0. eauto.
-    - constructor.
-      apply IHe0_1; eauto. eapply scope_ext_app. eauto.
-      apply IHe0_2; eauto. eapply scope_ext_app. eauto.
-  * split; intros. inversion H. subst. simpl. inversion H. 2: inversion H1. subst.
-    constructor. 
-    eapply IHe0_1; auto. eapply IHe0_2; auto.
-  * split; intros. inversion H. subst. simpl. inversion H. 2: inversion H1. subst.
-    constructor. 
-    eapply IHe0_1; auto. eapply IHe0_2; auto. eapply IHe0_3; auto.
-  * constructor. apply IHe0. apply IHe1.
-  * constructor.
-Unshelve. rewrite map_length in H1. auto.
+  firstorder.
 Qed.
 
-Theorem scope_funsub v : forall e,
-  (forall Γ, VAL (inr v::Γ) ⊢ e -> forall val, VAL Γ ⊢ val -> VAL Γ ⊢ (funsubst v val e)) /\
-  (forall Γ, EXP (inr v::Γ) ⊢ e -> forall val, EXP Γ ⊢ val -> EXP Γ ⊢ (funsubst v val e)).
+Hint Resolve renscope_id.
+
+Lemma scope_idsubst Γ : SUBSCOPE Γ ⊢ idsubst ∷ Γ.
 Proof.
-  einduction e using Exp_ind2 with 
-  (Q := fun l => Forall (fun e => (forall Γ, VAL (inr v::Γ) ⊢ e -> forall val, VAL Γ ⊢ val -> VAL Γ ⊢ (funsubst v val e)) /\
-  (forall Γ, EXP (inr v::Γ) ⊢ e -> forall val, EXP Γ ⊢ val -> EXP Γ ⊢ (funsubst v val e))) l); intros.
-  * split; intros; simpl; constructor. constructor.
-  * split; intros. inversion H.
-    inversion H2. congruence. simpl. subst. constructor. auto.
-    inversion H. inversion H1. inversion H4. congruence.
-      simpl. constructor. constructor. auto.
-  * split; intros; simpl; break_match_goal; auto. 
-    - inversion H. constructor.
-      inversion H2. subst. apply funid_eqb_neq in Heqb. inversion H3. subst. congruence. auto.
-    - inversion H. inversion H1. subst. inversion H4. inversion H2. subst.
-      rewrite funid_eqb_refl in Heqb. congruence.
-      constructor. constructor. auto.
-  * split; intros; inversion H; subst; simpl; constructor. 2: constructor.
-    - apply IHe0. rewrite app_comm_cons. auto. apply scope_ext_app. constructor. auto.
-    - inversion H1. subst. apply IHe0. rewrite app_comm_cons. auto.
-      apply scope_ext_app. auto.
-  * split; intros; inversion H; subst; simpl; break_match_goal.
-    - apply funid_eqb_eq in Heqb. subst. constructor. rewrite <- app_comm_cons in H2.
-      eapply scope_duplicate. 2: exact H2.
-      apply in_app_iff. right. apply in_app_iff. left. constructor. auto.
-    - constructor. apply IHe0. rewrite app_comm_cons. auto.
-      apply scope_ext_app. constructor. auto.
-    - inversion H1. subst. apply funid_eqb_eq in Heqb. subst.
-      constructor. constructor. rewrite <- app_comm_cons in H3.
-      eapply scope_duplicate. 2: exact H3.
-      apply in_app_iff. right. apply in_app_iff. left. constructor. auto.
-    - constructor. constructor. inversion H1. subst.
-      apply IHe0. rewrite app_comm_cons. auto.
-      apply scope_ext_app. auto.
-  * split; intros. inversion H.
-    simpl. inversion H. 2: inversion H1. subst. constructor.
-    - apply IHe0. auto. auto.
-    - rewrite indexed_to_forall in IHe1.
-      intros. epose (IHe1 i _). destruct a. clear H2 IHe1. Search map nth.
-      replace (ELit 0) with ((funsubst v val) (ELit 0)). rewrite map_nth. apply H5.
-      apply H4. rewrite map_length in H1. auto. auto. reflexivity.
-  * split; intros; inversion H; subst.
-    - simpl. constructor.
-      apply IHe0_1; eauto.
-      apply IHe0_2; eauto.
-      eapply scope_ext_app in H0. eauto.
-    - inversion H1.
-  * split; intros; inversion H. subst.
-    simpl. break_match_goal.
-    - constructor. apply funid_eqb_eq in Heqb. subst. rewrite <- app_comm_cons in H3.
-      eapply scope_duplicate. 2: exact H3. apply in_app_iff. right.
-      apply in_app_iff. left. constructor. auto.
-      apply funid_eqb_eq in Heqb. subst. rewrite <- app_comm_cons in H6.
-      eapply scope_duplicate. 2: exact H6. apply in_app_iff. intuition.
-    - apply funid_eqb_neq in Heqb. constructor.
-      apply IHe0_1. try rewrite app_comm_cons; eauto.
-      apply scope_ext_app. auto.
-      apply IHe0_2. rewrite app_comm_cons; auto.
-      apply scope_ext_app. auto.
-    - inversion H1.
-  * split; intros. inversion H. subst. simpl. inversion H. 2: inversion H1. subst.
-    constructor. 
-    eapply IHe0_1; auto. eapply IHe0_2; auto.
-  * split; intros. inversion H. subst. simpl. inversion H. 2: inversion H1. subst.
-    constructor. 
-    eapply IHe0_1; auto. eapply IHe0_2; auto. eapply IHe0_3; auto.
-  * constructor. apply IHe0. apply IHe1.
-  * constructor.
-Unshelve. rewrite map_length in H1. auto.
+  firstorder.
 Qed.
 
-Corollary scope_subst v : forall e,
-  (forall Γ, VAL (v::Γ) ⊢ e -> forall val, VAL Γ ⊢ val -> VAL Γ ⊢ (subst v val e)) /\
-  (forall Γ, EXP (v::Γ) ⊢ e -> forall val, EXP Γ ⊢ val -> EXP Γ ⊢ (subst v val e)).
+Hint Resolve scope_idsubst.
+
+Lemma upren_scope : forall Γ Γ' ξ,
+  RENSCOPE Γ ⊢ ξ ∷ Γ' ->
+  RENSCOPE (S Γ) ⊢ upren ξ ∷ (S Γ').
 Proof.
-  destruct v.
-  - apply scope_sub.
-  - apply scope_funsub.
+  intros.
+  unfold renscoped in *.
+  intros.
+  revert ξ Γ Γ' H H0.
+  induction v;
+    intros;
+    simpl;
+    firstorder using Nat.succ_lt_mono.
+    lia.
+  apply -> Nat.succ_lt_mono. apply H. lia.
 Qed.
-*)
-Theorem scope_duplicate_rev e :
-  (forall Γ v, In v Γ -> EXP Γ ⊢ e -> EXP v::Γ ⊢ e) /\
-  (forall Γ v, In v Γ -> VAL Γ ⊢ e -> VAL v::Γ ⊢ e).
+
+Lemma uprenn_scope : forall Γ'' Γ Γ' ξ,
+  RENSCOPE Γ ⊢ ξ ∷ Γ' ->
+  RENSCOPE (Γ'' + Γ) ⊢ uprenn Γ'' ξ ∷ (Γ'' + Γ').
 Proof.
-  einduction e using Exp_ind2 with 
-      (Q := fun l => Forall (fun e => 
-        (forall Γ v, In v Γ -> EXP Γ ⊢ e -> EXP (v::Γ) ⊢ e) /\
-        (forall Γ v, In v Γ -> VAL Γ ⊢ e -> VAL (v::Γ) ⊢ e)) l); intros.
-  * repeat constructor.
-  * split; intros.
-    - inversion H0. subst. constructor. constructor. constructor 2.
-      inversion H1. auto.
-    - inversion H0. constructor. constructor 2. subst. auto.
-  * split; intros. 
-    - inversion H0. subst. constructor. constructor. constructor 2.
-      inversion H1. auto.
-    - inversion H0. constructor. constructor 2. subst. auto.
-  * split; intros. 
-    - constructor. constructor. inversion H0. inversion H1. subst.
-      rewrite <- app_comm_cons. apply IHe0; auto. apply in_or_app. left.
-      auto.
-    - constructor. inversion H0. subst.
-      rewrite <- app_comm_cons. apply IHe0; auto. apply in_or_app. left.
-      auto.
-  * split; intros. 
-    - constructor. constructor. inversion H0. inversion H1. subst.
-      rewrite <- app_comm_cons . apply IHe0; auto. apply in_or_app. left.
-      auto.
-    - constructor. inversion H0. subst.
-      rewrite <- app_comm_cons. apply IHe0; auto. apply in_or_app. left.
-      auto.
-  * split; intros; inversion H0. 2: inversion H1. subst. rewrite indexed_to_forall in IHe1.
-    constructor.
-    - eapply IHe0; eauto.
-    - intros. eapply IHe1; eauto.
-  * split; intros; inversion H0. 2: inversion H1. subst. constructor.
-    - eapply IHe0_1. exact H. auto.
-    - rewrite <- app_comm_cons. eapply IHe0_2. 2: exact H5.
-      apply in_or_app. left. auto.
-  * split; intros; inversion H0. 2: inversion H1. subst. constructor.
-    - eapply IHe0_1. apply in_or_app. left. eauto. auto.
-    - rewrite <- app_comm_cons. eapply IHe0_2. apply in_or_app. left. eauto. auto.
-  * split; intros; inversion H0. 2: inversion H1. subst. constructor.
-    - eapply IHe0_1; eauto.
-    - eapply IHe0_2; eauto.
-  * split; intros; inversion H0. 2: inversion H1. subst. constructor.
-    - eapply IHe0_1; eauto.
-    - eapply IHe0_2; eauto.
-    - eapply IHe0_3; eauto.
+  induction Γ''; intros.
+  * repeat rewrite Nat.add_0_l. apply H.
+  * repeat rewrite Nat.add_succ_l. apply upren_scope. apply IHΓ''. auto.
+Qed.
+
+Hint Resolve upren_scope.
+Hint Resolve uprenn_scope.
+
+Theorem idren_is_id : forall e,
+  rename id e = e.
+Proof.
+  induction e; intros.
+  (* TODO *)
+Admitted.
+
+Theorem idsubst_is_id : forall e,
+  subst idsubst e = e.
+Proof.
+  induction e; intros.
+  (* TODO *)
+Admitted.
+
+Lemma ren_preserves_scope : forall e Γ,
+    (EXP Γ ⊢ e <->
+     forall Γ' ξ,
+       RENSCOPE Γ ⊢ ξ ∷ Γ' ->
+       EXP Γ' ⊢ rename ξ e) /\
+    (VAL Γ ⊢ e <->
+     forall Γ' ξ,
+       RENSCOPE Γ ⊢ ξ ∷ Γ' ->
+       VAL Γ' ⊢ rename ξ e).
+Proof.
+  induction e using Exp_ind2 with
+  (Q := fun l => Forall (fun e => forall Γ,(EXP Γ ⊢ e <->
+     forall Γ' ξ,
+       RENSCOPE Γ ⊢ ξ ∷ Γ' ->
+       EXP Γ' ⊢ rename ξ e) /\
+    (VAL Γ ⊢ e <->
+     forall Γ' ξ,
+       RENSCOPE Γ ⊢ ξ ∷ Γ' ->
+       VAL Γ' ⊢ rename ξ e)) l);
+  try (intros Γ;
+  split;
+  split;
+  intros; cbn; unfold renscoped in *).
+  1-4: constructor. 1-2: constructor.
+  1, 5, 7: repeat constructor; try apply H0; try inversion H; try inversion H1; auto.
+  all: (* this solves around half the goals *)
+    try (specialize (H Γ id (renscope_id _)); rewrite idren_is_id in H; apply H).
+  all: try (inversion H; inversion H1).
+  * constructor. apply H0. inversion H. auto.
+  * constructor. constructor. inversion H; inversion H1. subst.
+    eapply IHe; eauto. intros. pose (uprenn_scope (length vl) _ Γ' ξ H0 v H2). auto.
+  * constructor. inversion H. subst.
+    eapply IHe; eauto. intros. pose (uprenn_scope (length vl) _ Γ' ξ H0 v H1). auto.
+  * constructor. constructor. inversion H; inversion H1. subst.
+    eapply IHe; eauto. intros. pose (uprenn_scope (S (length vl)) _ Γ' ξ H0 v H2). auto.
+  * constructor. inversion H. subst.
+    eapply IHe; eauto. intros. pose (uprenn_scope (S (length vl)) _ Γ' ξ H0 v H1). auto.
+  * subst. constructor.
+    - eapply IHe; eauto.
+    - intros. Search Forall. rewrite indexed_to_forall in IHe0.
+      replace (ELit 0) with (rename ξ (ELit 0)) by auto.
+      rewrite map_nth. rewrite map_length in H1. eapply IHe0; eauto.
+  * subst. constructor.
+    - eapply IHe1; eauto.
+    - eapply IHe2; eauto. intros. eapply upren_scope; eauto.
+  * subst. constructor.
+    - eapply IHe1; eauto. intros. eapply upren_scope; eauto.
+    - eapply IHe2; eauto. intros. eapply upren_scope; eauto.
+  * subst. constructor.
+    - eapply IHe1; eauto.
+    - eapply IHe2; eauto.
+  * subst. constructor.
+    - eapply IHe1; eauto.
+    - eapply IHe2; eauto.
+    - eapply IHe3; eauto.
   * constructor; eauto.
   * constructor.
 Qed.
-(* 
-Corollary scope_subst_in v : forall e,
-  (forall Γ, In v Γ -> 
-    VAL Γ ⊢ e -> forall val, VAL Γ ⊢ val -> VAL Γ ⊢ (subst v val e)) /\
-  (forall Γ, In v Γ ->
-    EXP Γ ⊢ e -> forall val, EXP Γ ⊢ val -> EXP Γ ⊢ (subst v val e)).
-Proof.
-  intros; split; intros.
-  * apply scope_subst; auto. eapply scope_duplicate_rev in H; eauto.
-  * apply scope_subst; auto. pose (scope_duplicate_rev e). destruct a. apply H2; eauto.
-Qed. *)
 
-Definition subscoped (l l' : list VarFunId) (ξ : Substitution) : Prop :=
-  forall v, In v l -> VAL l' ⊢ ξ v.
-
-(* Corollary scope_subst_list Γ' : forall Γ e,
-  (VAL (Γ ++ Γ') ⊢ e -> forall vals, length vals = length Γ' -> subscoped Γ vals -> VAL Γ ⊢ (subst_list Γ' vals e)) /\
-  (EXP (Γ ++ Γ') ⊢ e -> forall vals, length vals = length Γ' -> subscoped Γ vals -> EXP Γ ⊢ (subst_list Γ' vals e)).
+Lemma ren_preserves_scope_exp : forall e Γ,
+    (EXP Γ ⊢ e <->
+     forall Γ' ξ,
+       RENSCOPE Γ ⊢ ξ ∷ Γ' ->
+       EXP Γ' ⊢ rename ξ e).
 Proof.
-  induction Γ'; split; intros.
-  1-2: rewrite app_nil_r in H; unfold subst_list; simpl; auto.
-  * unfold subscoped in H1. apply eq_sym, element_exist in H0 as EE. destruct EE, H2.
-    subst. unfold subst_list. simpl.
-    replace (fold_left (fun (acc : Exp) '(v, val) => subst v val acc) (combine Γ' x0) (subst a x e)) with (subst_list Γ' x0 (subst a x e)). 2: reflexivity.
-    specialize (IHΓ' Γ (subst a x e)). destruct IHΓ'.
-    inversion H0.
-    epose (H2 _ x0 (eq_sym H5) _). auto.
-  * unfold subscoped in H1. apply eq_sym, element_exist in H0 as EE. destruct EE, H2.
-    subst. unfold subst_list. simpl.
-    replace (fold_left (fun (acc : Exp) '(v, val) => subst v val acc) (combine Γ' x0) (subst a x e)) with (subst_list Γ' x0 (subst a x e)). 2: reflexivity.
-    specialize (IHΓ' Γ (subst a x e)). destruct IHΓ'.
-    inversion H0.
-    epose (H3 _ x0 (eq_sym H5) _). auto.
-Unshelve.
-  2, 4: intro; intros; apply (H1 (S i)); simpl; lia.
-  - apply scope_subst; eauto.
-    + eapply perm_scoped. exact H. apply Permutation_sym, Permutation_middle.
-    + specialize (H1 0 (Nat.lt_0_succ _)).
-      simpl in H1. apply scope_ext_app. auto.
-  - apply scope_subst; eauto.
-    + eapply perm_scoped. exact H. apply Permutation_sym, Permutation_middle.
-    + specialize (H1 0 (Nat.lt_0_succ _)).
-      simpl in H1. apply scope_ext_app. auto. constructor. auto.
+  intros.
+  apply ren_preserves_scope.
 Qed.
 
-
-Corollary scope_subst_list_closed Γ : forall e,
-  (VAL Γ ⊢ e -> forall vals, length vals = length Γ -> subscoped [] vals -> VALCLOSED (subst_list Γ vals e)) /\
-  (EXP Γ ⊢ e -> forall vals, length vals = length Γ -> subscoped [] vals -> EXPCLOSED (subst_list Γ vals e)).
+Lemma ren_preserves_scope_val : forall e Γ,
+    (VAL Γ ⊢ e <->
+     forall Γ' ξ,
+       RENSCOPE Γ ⊢ ξ ∷ Γ' ->
+       VAL Γ' ⊢ rename ξ e).
 Proof.
-  intros. pose (scope_subst_list Γ []). simpl in a. auto.
-Qed. *)
-Fixpoint create_list (e : Exp) (n : nat) :=
-match n with
-| 0 => []
-| S n' => e :: create_list e n'
-end.
+  intros.
+  apply ren_preserves_scope.
+Qed.
 
-(* Corollary subst_in_list :
-  forall l ξ v e, In (v, e) l -> ξ[[ ::= l]] v = e.
+Lemma up_val : forall Γ v (ξ : Substitution),
+  match ξ v with
+  | inl exp => VAL Γ ⊢ exp
+  | inr num => num < Γ
+  end ->
+  match up_subst ξ (S v) with
+  | inl exp => VAL S Γ ⊢ exp
+  | inr num => num < S Γ
+  end.
 Proof.
-  induction l; intros.
-  * inversion H.
-  * unfold extend_subst_list. simpl. destruct a.
-    replace (fold_right (fun '(x, e1) (ξ' : Substitution) => ξ' [[x ::= e1]]) ξ l [[v0 ::= e0]]) with (ξ[[ ::= l]][[v0 ::= e0]]) by reflexivity.
-    epose (var_funid_eq_dec v v0).
-    destruct s.
-    - inversion e1. subst. apply subst_in. 
-    - inversion H.
-      + congruence.
-      + rewrite subst_not_in; auto. apply IHl.
-Qed. *)
+  intros. unfold up_subst.
+  break_match_hyp.
+  * apply -> ren_preserves_scope_val; eauto.
+    intro. intros. lia.
+  * lia.
+Qed.
 
-Theorem var_not_closed1 v : ~ VALCLOSED (EVar v).
+Lemma up_scope : forall Γ Γ' ξ,
+  SUBSCOPE Γ ⊢ ξ ∷ Γ' ->
+  SUBSCOPE (S Γ) ⊢ up_subst ξ ∷ (S Γ').
+Proof.
+  intros.
+  unfold subscoped in *.
+  intros.
+  destruct v; intros.
+  * simpl. lia.
+  * simpl. break_match_goal. break_match_hyp.
+    - inversion Heqs. eapply ren_preserves_scope_val with (Γ:= Γ'); eauto.
+      + epose (H v _). rewrite Heqs0 in y. auto. Unshelve. lia.
+      + intro. intros. lia.
+    - inversion Heqs.
+    - break_match_hyp.
+      + inversion Heqs.
+      + inversion Heqs. subst. epose (H v _). rewrite Heqs0 in y. lia. Unshelve. lia.
+Qed.
+
+Hint Resolve up_scope.
+
+Lemma upn_scope : forall n Γ Γ' ξ,
+  SUBSCOPE Γ ⊢ ξ ∷ Γ' ->
+  SUBSCOPE (n + Γ) ⊢ upn n ξ ∷ (n + Γ').
+Proof.
+  induction n; intros.
+  * repeat rewrite Nat.add_0_l. apply H.
+  * repeat rewrite Nat.add_succ_l. apply up_scope. apply IHn. auto.
+Qed.
+
+Hint Resolve upn_scope.
+
+Lemma cons_scope : forall v Γ Γ' ξ,
+    VAL Γ' ⊢ v ->
+    SUBSCOPE Γ ⊢ ξ ∷ Γ' ->
+    SUBSCOPE (S Γ) ⊢ v.:ξ ∷ Γ'.
+Proof.
+  intros.
+  unfold subscoped in *.
+  intros. destruct v0.
+  * simpl. auto.
+  * simpl. apply H0. lia.
+Qed.
+
+Hint Resolve cons_scope.
+
+(** Substitution is scope-preserving. *)
+Lemma sub_preserves_scope : forall e Γ,
+    (EXP Γ ⊢ e <->
+     forall Γ' ξ,
+       SUBSCOPE Γ ⊢ ξ ∷ Γ' ->
+       EXP Γ' ⊢ e.[ξ]) /\
+    (VAL Γ ⊢ e <->
+     forall Γ' ξ,
+       SUBSCOPE Γ ⊢ ξ ∷ Γ' ->
+       VAL Γ' ⊢ e.[ξ]).
+Proof.
+  induction e using Exp_ind2 with
+  (Q := fun l => forall Γ,
+  Forall (fun e => (EXP Γ ⊢ e <->
+     forall Γ' ξ,
+       SUBSCOPE Γ ⊢ ξ ∷ Γ' ->
+       EXP Γ' ⊢ e.[ξ]) /\
+    (VAL Γ ⊢ e <->
+     forall Γ' ξ,
+       SUBSCOPE Γ ⊢ ξ ∷ Γ' ->
+       VAL Γ' ⊢ e.[ξ])) l);
+    try intros Γ;
+    try split;
+    try split;
+    intros.
+  all: cbn; unfold subscoped in *.
+  1-4: repeat constructor.
+  all: try (inversion H); try inversion H1; subst. (* cleaup contradictions *)
+  (* prove backward directions: *)
+  all: try (specialize (H Γ idsubst (scope_idsubst _)); rewrite idsubst_is_id in H; auto).
+  (* forward: *)
+  * specialize (H0 n H4). break_match_goal.
+    - constructor. auto.
+    - constructor. constructor. auto.
+  * specialize (H0 n H2). break_match_goal.
+    - auto.
+    - constructor. auto.
+  * specialize (H0 n H4). break_match_goal.
+    - constructor. auto.
+    - constructor. constructor. auto.
+  * specialize (H0 n H2). break_match_goal.
+    - auto.
+    - constructor. auto.
+  * constructor. constructor. eapply IHe; eauto. intros.
+    eapply upn_scope; eauto.
+  * constructor. eapply IHe; eauto. intros.
+    eapply upn_scope; eauto.
+  * constructor. constructor. eapply IHe; eauto. intros.
+    eapply up_scope; eauto.
+  * constructor. eapply IHe; eauto. intros.
+    eapply up_scope; eauto.
+  * constructor.
+    - eapply IHe; eauto.
+    - replace (ELit 0) with (subst ξ (ELit 0)) by reflexivity. intros.
+      specialize (IHe0 Γ).
+      rewrite map_nth. rewrite indexed_to_forall in IHe0. rewrite map_length in H1.
+      eapply IHe0; eauto.
+  * constructor.
+    - eapply IHe1; eauto.
+    - eapply IHe2; eauto. apply up_scope. auto.
+  * constructor.
+    - eapply IHe1; eauto. apply up_scope. auto.
+    - eapply IHe2; eauto. apply up_scope. auto.
+  * constructor.
+    - eapply IHe1; eauto.
+    - eapply IHe2; eauto.
+  * constructor.
+    - eapply IHe1; eauto.
+    - eapply IHe2; eauto.
+    - eapply IHe3; eauto.
+  * constructor; auto.
+  * constructor.
+Qed.
+
+Lemma sub_preserves_scope_exp : forall e Γ,
+    EXP Γ ⊢ e <->
+    forall Γ' ξ,
+      SUBSCOPE Γ ⊢ ξ ∷ Γ' ->
+      EXP Γ' ⊢ e.[ξ].
+Proof.
+  intros.
+  apply sub_preserves_scope.
+Qed.
+
+Lemma sub_preserves_scope_val : forall e Γ,
+    VAL Γ ⊢ e <->
+    forall Γ' ξ,
+      SUBSCOPE Γ ⊢ ξ ∷ Γ' ->
+      VAL Γ' ⊢ e.[ξ].
+Proof.
+  intros.
+  apply sub_preserves_scope.
+Qed.
+
+Module SUB_IMPLIES_SCOPE.
+  Definition magic_ξ (Γ Γ' : nat) (n : nat) : Exp + nat :=
+    if Compare_dec.lt_dec n Γ
+    then if Compare_dec.lt_dec n Γ'
+         then inr n
+         else inl (ELit 0)
+    else inr Γ'(* inl (EVar Γ' "x"%string) *).
+
+  Lemma magic_ξ_scope : forall Γ Γ', SUBSCOPE Γ ⊢ magic_ξ Γ Γ' ∷ Γ'.
+  Proof.
+    unfold subscoped.
+    intros.
+    unfold magic_ξ.
+    repeat destruct Compare_dec.lt_dec; try congruence.
+    constructor.
+  Qed.
+
+  Lemma up_magic Γ Γ': up_subst (magic_ξ Γ Γ') = magic_ξ (S Γ) (S Γ').
+  Proof.
+    extensionality x.
+    unfold magic_ξ, up_subst.
+    destruct x; cbn; auto.
+    repeat destruct Compare_dec.lt_dec; auto; lia.
+  Qed.
+
+  Lemma magic_ξ_implies_scope : forall e Γ Γ',
+      (EXP Γ' ⊢ e.[magic_ξ Γ Γ'] ->
+       EXP Γ ⊢ e) /\
+      (VAL Γ' ⊢ e.[magic_ξ Γ Γ'] ->
+       VAL Γ ⊢ e).
+  Proof.
+    induction e;
+      intros Γ Γ';
+      split;
+      intros;
+      cbn in H;
+      try invert_scoped H;
+      try solve
+          [constructor;
+           let e := match goal with
+                    | [ |- EXP _ ⊢ ?e ] => e
+                    | [ |- VAL _ ⊢ ?e ] => e
+                    end in
+           match goal with
+           | [IHe : forall (Γ Γ' : Env), (_ -> EXP Γ ⊢ e) /\ (_ -> VAL Γ ⊢ e),
+                H : VAL _ ⊢ e.[magic_ξ Γ Γ'] |- _ ] =>
+             eapply IHe in H; try eassumption; auto
+           | [IHe : forall (Γ Γ' : Env), (_ -> EXP Γ ⊢ e) /\ (_ -> VAL Γ ⊢ e),
+                H : EXP _ ⊢ e.[magic_ξ Γ Γ'] |- _ ] =>
+             eapply IHe in H; try eassumption; auto
+           end];
+    auto.
+    - cbn in *.
+      unfold magic_ξ in H.
+      repeat destruct lt_dec;
+        auto.
+      inversion H; subst.
+      inversion H0.
+      auto.
+    - cbn in *.
+      unfold magic_ξ in H.
+      repeat destruct lt_dec;
+        auto.
+      inversion H.
+      auto.
+    - constructor.
+      constructor.
+      eapply IHe.
+      rewrite <- up_magic.
+      eauto.
+    - constructor.
+      eapply IHe.
+      rewrite <- up_magic.
+      eauto.
+    - constructor;
+        firstorder idtac.
+      eapply IHe0.
+      rewrite <- up_magic.
+      eauto.
+  Qed.
+
+  Lemma sub_implies_scope_exp : forall e Γ Γ',
+      (forall ξ, SUBSCOPE Γ ⊢ ξ ∷ Γ' -> EXP Γ' ⊢ e.[ξ]) ->
+      EXP Γ ⊢ e.
+  Proof.
+    intros;
+    eapply magic_ξ_implies_scope;
+    apply H;
+    apply magic_ξ_scope.
+  Qed.
+
+  Lemma sub_implies_scope_val : forall e Γ Γ',
+      (forall ξ, SUBSCOPE Γ ⊢ ξ ∷ Γ' -> VAL Γ' ⊢ e.[ξ]) ->
+      VAL Γ ⊢ e.
+  Proof.
+    intros;
+    eapply magic_ξ_implies_scope;
+    apply H;
+    apply magic_ξ_scope.
+  Qed.
+
+  Definition magic_ξ_2 Γ' :=
+    fun n =>
+      if lt_dec n Γ'
+      then Var n
+      else if Nat.eq_dec n Γ'
+           then Const 0
+           else Var (pred n).
+
+  Lemma up_magic_2 : forall Γ,
+      up (magic_ξ_2 Γ) = magic_ξ_2 (S Γ).
+  Proof.
+    intros.
+    unfold magic_ξ_2.
+    extensionality x.
+    unfold up.
+    unfold ".:".
+    destruct x; auto.
+    simpl.
+    unfold Init.Nat.pred.
+    repeat destruct lt_dec;
+      destruct (Nat.eq_dec x Γ);
+      destruct x;
+      subst;
+      cbn;
+      auto.
+  Qed.
+
+  Lemma magic_const : magic_ξ_2 0 = Const 0 .: ids.
+  Proof.
+    unfold magic_ξ_2.
+    extensionality x.
+    destruct lt_dec; auto.
+    destruct Nat.eq_dec; subst; auto.
+    destruct x; cbn; auto.
+  Qed.
+
+  Lemma foo : forall e Γ',
+      (EXP Γ' ⊢ e.[magic_ξ_2 Γ'] ->
+       e.[magic_ξ (S Γ') Γ'] = e.[magic_ξ_2 Γ']) /\
+      (VAL Γ' ⊢ e.[magic_ξ_2 Γ'] ->
+       e.[magic_ξ (S Γ') Γ'] = e.[magic_ξ_2 Γ']).
+  Proof.
+    induction e;
+      split;
+      intros Hscope;
+      cbn;
+      cbn in Hscope;
+      try invert_scoped Hscope;
+      auto;
+      try rewrite up_magic_2 in *;
+      try rewrite up_magic in *;
+      try solve
+          [repeat
+             match goal with
+             | [ IHe : forall (Γ' : Env), (EXP Γ' ⊢ ?e.[_] -> _) /\ (VAL Γ' ⊢ ?e.[_] -> _),
+                   H : VAL _ ⊢ ?e.[_]
+                   |- _] => apply IHe in H
+             | [ IHe : forall (Γ' : Env), (EXP Γ' ⊢ ?e.[_] -> _) /\ (VAL Γ' ⊢ ?e.[_] -> _),
+                   H : EXP _ ⊢ ?e.[_]
+                   |- _] => apply IHe in H
+             end;
+           f_equal;
+           auto].
+    - unfold magic_ξ, magic_ξ_2 in *;
+        cbn in *;
+        repeat destruct lt_dec; auto;
+          destruct (Nat.eq_dec v Γ'); auto;
+            destruct v, Γ';
+            inversion Hscope;
+            try inversion H;
+            subst;
+            cbn;
+            auto.
+    - asimpl in Hscope.
+      unfold magic_ξ, magic_ξ_2 in *.
+      repeat destruct lt_dec;
+        repeat destruct Nat.eq_dec;
+        inversion Hscope;
+        auto.
+  Qed.
+
+  Lemma bar : forall e,
+      (ECLOSED e.[Const 0/] ->
+       e.[magic_ξ 1 0] = e.[Const 0 .: ids]) /\
+      (VCLOSED e.[Const 0/] ->
+       e.[magic_ξ 1 0] = e.[Const 0 .: ids]).
+  Proof.
+    intros.
+    rewrite <- magic_const.
+    apply foo.
+  Qed.
+
+  Lemma sub_implies_scope_exp_1 : forall e,
+      ECLOSED e.[Const 0/] ->
+      EXP 1 ⊢ e.
+  Proof.
+    intros;
+      eapply magic_ξ_implies_scope.
+    destruct (bar e).
+    rewrite H0; auto.
+  Qed.
+
+  Lemma sub_implies_scope_val_1 : forall e,
+      VCLOSED e.[Const 0/] ->
+      VAL 1 ⊢ e.
+  Proof.
+    intros;
+      eapply magic_ξ_implies_scope.
+    destruct (bar e).
+    rewrite H1; auto.
+  Qed.
+End SUB_IMPLIES_SCOPE.
+
+Definition sub_implies_scope_exp := SUB_IMPLIES_SCOPE.sub_implies_scope_exp.
+Definition sub_implies_scope_val := SUB_IMPLIES_SCOPE.sub_implies_scope_val.
+Definition sub_implies_scope_exp_1 := SUB_IMPLIES_SCOPE.sub_implies_scope_exp_1.
+Definition sub_implies_scope_val_1 := SUB_IMPLIES_SCOPE.sub_implies_scope_val_1.
+
+Lemma upn_Var : forall (Γ : Env) (ξ : var -> Expr) (v : var),
+    v < Γ -> upn Γ ξ v = Var v.
+Proof.
+  intros Γ ξ.
+  induction Γ;
+    intros.
+  + auto.
+  + rewrite iterate_S.
+    destruct v;
+      asimpl;
+      auto.
+    rewrite IHΓ;
+      auto.
+Qed.
+
+Lemma scoped_ignores_sub : forall e Γ ξ,
+     (EXP Γ ⊢ e -> e.[upn Γ ξ] = e) /\
+     (VAL Γ ⊢ e -> e.[upn Γ ξ] = e).
+Proof.
+  induction e;
+    cbn;
+    split;
+    intros;
+    invert_scoped H;
+    auto using upn_Var;
+    try solve
+        [repeat
+           match goal with
+           | [ IHe : forall (Γ : Env) (ξ : var -> Expr), (EXP Γ ⊢ ?e -> _) /\ (VAL Γ ⊢ ?e -> _),
+                 H : VAL _ ⊢ ?e
+                 |- _] => eapply IHe in H
+           | [ IHe : forall (Γ : Env) (ξ : var -> Expr), (EXP Γ ⊢ ?e -> _) /\ (VAL Γ ⊢ ?e -> _),
+                 H : EXP _ ⊢ ?e
+                 |- _] => eapply IHe in H
+           end;
+         f_equal;
+         eauto].
+Qed.
+
+Lemma escoped_ignores_sub : forall e Γ ξ,
+    EXP Γ ⊢ e -> e.[upn Γ ξ] = e.
+Proof.  
+  intros.
+  eapply scoped_ignores_sub in H.
+  eauto.
+Qed.
+Hint Resolve escoped_ignores_sub.
+
+Lemma vscoped_ignores_sub : forall e Γ ξ,
+    VAL Γ ⊢ e -> e.[upn Γ ξ] = e.
+Proof.
+  intros.
+  eapply scoped_ignores_sub in H.
+  eauto.
+Qed.
+Hint Resolve vscoped_ignores_sub.
+
+Lemma eclosed_ignores_sub : forall e ξ,
+     ECLOSED e -> e.[ξ] = e.
+Proof.
+  intros.
+  replace (e.[ξ]) with (e.[upn 0 ξ])
+    by (rewrite upn0; auto).
+  auto.
+Qed.
+Hint Resolve eclosed_ignores_sub.
+
+Lemma vclosed_ignores_sub : forall e ξ,
+     VCLOSED e -> e.[ξ] = e.
+Proof.
+  intros.
+  replace (e.[ξ]) with (e.[upn 0 ξ])
+    by (rewrite upn0; auto).
+  auto.
+Qed.
+Hint Resolve vclosed_ignores_sub.
+
+Lemma eclosed_sub_closed : forall v ξ,
+    ECLOSED v -> ECLOSED v.[ξ].
+Proof.
+  intros.
+  rewrite eclosed_ignores_sub;
+    auto.
+Qed.
+Hint Resolve eclosed_sub_closed.
+
+Lemma vclosed_sub_closed : forall v ξ,
+    VCLOSED v -> VCLOSED v.[ξ].
+Proof.
+  intros.
+  rewrite vclosed_ignores_sub;
+    auto.
+Qed.
+Hint Resolve vclosed_sub_closed.
+
+(* Continuations *)
+
+Inductive Kont : Type :=
+| Knil : Kont
+| Kcons : Expr -> Kont -> Kont.
+
+Infix "-:" := Kcons (at level 60, right associativity).
+
+Lemma Kont_eq_dec : forall (K K' : Kont),
+    decidable (K = K').
+Proof.
+  unfold decidable.
+  induction K;
+    destruct K';
+    intros;
+    try solve [intuition auto].
+  destruct (Expr_eq_dec e e0);
+    subst;
+    revgoals.
+  { right.
+    contradict n.
+    inversion n; subst; auto.
+  }
+  specialize (IHK K').
+  inversion IHK; subst.
+  + left; auto.
+  + right.
+    contradict H.
+    inversion H.
+    auto.
+Qed.
+
+Reserved Notation "'KCLOSED' K" (at level 69).
+
+Inductive KontScoped : forall K, Prop :=
+| KontScoped_nil :
+    KCLOSED Knil
+| KontScoped_cons : forall K e,
+    EXP 1 ⊢ e ->
+    KCLOSED K ->
+    KCLOSED e -: K
+where
+"'KCLOSED' K" := (KontScoped K).
+
+Hint Constructors KontScoped.
+
+Theorem var_not_closed1 n v : ~ VALCLOSED (EVar n v).
 Proof. intro. inversion H. inversion H1. Qed.
 
 Hint Resolve var_not_closed1.
 
-Theorem var_not_closed2 v : ~ EXPCLOSED (EVar v).
+Theorem var_not_closed2 n v : ~ EXPCLOSED (EVar n v).
 Proof. intro. inversion H. eapply var_not_closed1. eauto. Qed.
 
 Hint Resolve var_not_closed2.
 
-Theorem funid_not_closed1 v : ~ VALCLOSED (EFunId v).
+Theorem funid_not_closed1 n f : ~ VALCLOSED (EFunId n f).
 Proof. intro. inversion H. inversion H1. Qed.
 
 Hint Resolve funid_not_closed1.
 
-Theorem funid_not_closed2 v : ~ EXPCLOSED (EFunId v).
+Theorem funid_not_closed2 n f : ~ EXPCLOSED (EFunId n f).
 Proof. intro. inversion H. eapply funid_not_closed1. eauto. Qed.
 
 Hint Resolve funid_not_closed2.
 
-Theorem restrict_in : forall l ξ v,
+(* Theorem restrict_in : forall l ξ v,
   In v l -> (ξ -- l) v = idsubst v.
 Proof.
   intros. unfold "--". apply in_list_sound in H. rewrite H. auto.
@@ -589,17 +913,16 @@ Theorem restrict_not_in : forall l ξ v,
   ~In v l -> (ξ -- l) v = ξ v.
 Proof.
   intros. unfold "--". apply not_in_list_sound in H. rewrite H. auto.
-Qed.
+Qed. *)
+
+
+
 
 Theorem subscoped_preserves_app : forall ξ Γ Γ',
-  subscoped Γ Γ' ξ -> (forall l, subscoped (Γ ++ l) (Γ' ++ l) (ξ -- l)).
+  subscoped Γ Γ' ξ -> (subscoped (S Γ) (S Γ') (up_subst ξ)).
 Proof.
-  intros. intro. intros. destruct (in_dec var_funid_eq_dec v l) eqn:P.
-  * rewrite restrict_in by auto. unfold idsubst.
-    destruct v; constructor; apply in_app_iff; right; auto.
-  * rewrite restrict_not_in by auto.
-    apply scope_ext_app. unfold subscoped in H. apply H.
-    apply in_app_iff in H0. destruct H0; auto. congruence.
+  intros. intro. intros. break_match_goal.
+  * unfold subscoped in H.
 Qed.
 
 Hint Resolve subscoped_preserves_app.
